

Maximum likelihood estimation for regression models

Ciaran Evans

Warmup

Work on the warmup activity (handout), then we will discuss as a class.

Warmup

Suppose that we have independent observations $(\mathbf{x}_1, Y_1), \dots, (\mathbf{x}_n, Y_n)$ from the model

$$Y_i | \mathbf{x}_i \sim N(\mathbf{x}_i^T \beta, \sigma_i^2).$$

Suppose that the variances $\sigma_1^2, \dots, \sigma_n^2$ are known. Show that the maximum likelihood estimator of β minimizes the weighted sum of squares

$$\begin{aligned} WSS(\beta) &= \sum_{i=1}^n w_i (Y_i - \mathbf{x}_i^T \beta)^2 = (\mathbf{y} - \mathbf{X}\beta)^T \mathbf{W}(\mathbf{y} - \mathbf{X}\beta) \\ L(\beta | \mathbf{y}, \mathbf{X}) &\propto \prod_{i=1}^n f(Y_i | \mathbf{x}_i, \beta) = \prod_{i=1}^n \frac{1}{\sqrt{2\pi\sigma_i^2}} \exp\left\{-\frac{1}{2\sigma_i^2} (Y_i - \mathbf{x}_i^T \beta)^2\right\} \\ &= \left(\prod_{i=1}^n \frac{1}{\sqrt{2\pi\sigma_i^2}} \right) \exp\left\{-\frac{1}{2} \sum_{i=1}^n \frac{1}{\sigma_i^2} (Y_i - \mathbf{x}_i^T \beta)^2\right\} \\ &= \left(\prod_{i=1}^n \frac{1}{\sqrt{2\pi\sigma_i^2}} \right) \exp\left\{-\frac{1}{2} \sum_{i=1}^n w_i (Y_i - \mathbf{x}_i^T \beta)^2\right\} \quad w_i = \frac{1}{\sigma_i^2} \\ &\quad \text{(inverse variance weighting)} \\ &\Rightarrow \text{maximizing } L \Leftrightarrow \text{minimizing } WSS! \end{aligned}$$

Maximum likelihood estimation and logistic regression

Let $(\mathbf{x}_1, Y_1), \dots, (\mathbf{x}_n, Y_n)$ be iid samples from the model

$$Y_i | \mathbf{x}_i \sim \text{Bernoulli}(p_i)$$

$$\log \left(\frac{p_i}{1 - p_i} \right) = \mathbf{x}_i^T \boldsymbol{\beta}$$

where the distribution of \mathbf{x}_i does not depend on $\boldsymbol{\beta}$.

$$\ell(\boldsymbol{\beta} | \mathbf{y}, \mathbf{X}) \stackrel{\text{(up to a constant)}}{=} \sum_{i=1}^n \left\{ Y_i \mathbf{x}_i^T \boldsymbol{\beta} - \log(1 + e^{\mathbf{x}_i^T \boldsymbol{\beta}}) \right\}$$

score function $\hookrightarrow U(\boldsymbol{\beta}) = \frac{\partial \ell}{\partial \boldsymbol{\beta}} = \mathbf{X}^T (\mathbf{y} - \mathbf{p})$

Newton's method

- ▶ Want β^* such that $U(\beta^*) = \mathbf{0}$
- ▶ Begin with initial estimate $\beta^{(0)}$
- ▶ Iterative updates:

$$\beta^{(r+1)} = \beta^{(r)} - \left(\mathbf{H}(\beta^{(r)}) \right)^{-1} U(\beta^{(r)})$$

$$\beta = (\beta_0, \dots, \beta_K)^T \in \mathbb{R}^{K+1}$$

$$u(\beta) = \frac{\partial \ell}{\partial \beta} = x^T (\mathbf{I} - \mathbf{p}) \in \mathbb{R}^{K+1}$$

$$\mathbf{H}(\beta) = \frac{\partial^2 \ell}{\partial \beta^2} \in \mathbb{R}^{(K+1) \times (K+1)}$$

Hessian

The Hessian

$$\mathbf{p} = \begin{pmatrix} p_1 \\ \vdots \\ p_n \end{pmatrix} \in \mathbb{R}^n$$

$$U(\beta) = \frac{\partial}{\partial \beta} \ell(\beta | \mathbf{y}, \mathbf{X}) = \mathbf{X}^T (\mathbf{y} - \mathbf{p})$$

$$\mathbf{H}(\beta) = \frac{\partial}{\partial \beta} U(\beta) = \frac{\partial}{\partial \beta} \mathbf{X}^T (\mathbf{y} - \mathbf{p}) = \left(-\frac{\partial \mathbf{p}}{\partial \beta} \right) \mathbf{X}$$

$$\frac{\partial \mathbf{p}}{\partial \beta} = \begin{bmatrix} \frac{\partial p_1}{\partial \beta} & \frac{\partial p_2}{\partial \beta} & \dots & \frac{\partial p_n}{\partial \beta} \end{bmatrix} \in \mathbb{R}^{(k+1) \times n}$$

$$p_i = \frac{e^{x_i^T \beta}}{1 + e^{x_i^T \beta}}$$

$$= g(u(\beta))$$

$$g(u) = \frac{e^u}{1 + e^u}$$

$$u(\beta) = x_i^T \beta$$

Chain rule: $\frac{\partial}{\partial \beta} g(u(\beta)) = g'(u(\beta)) \frac{\partial u(\beta)}{\partial \beta}$

$$g'(u) = \frac{e^u}{(1 + e^u)^2}$$

$$\frac{\partial u}{\partial \beta} = \frac{\partial}{\partial \beta} x_i^T \beta = x_i$$

$$\Rightarrow \frac{\partial p_i}{\partial \beta} = \frac{e^{x_i^T \beta}}{(1 + e^{x_i^T \beta})^2} x_i = p_i (1 - p_i) x_i$$

The Hessian

$$U(\beta) = \frac{\partial}{\partial \beta} \ell(\beta | \mathbf{y}, \mathbf{X}) = \mathbf{X}^T (\mathbf{y} - \mathbf{p})$$

$$\mathbf{H}(\beta) = \frac{\partial}{\partial \beta} U(\beta) = \frac{\partial}{\partial \beta} \mathbf{X}^T (\mathbf{y} - \mathbf{p}) = \left(-\frac{\partial \mathbf{p}}{\partial \beta} \right) \mathbf{X}$$

$$\frac{\partial \mathbf{p}}{\partial \beta} = \begin{bmatrix} \frac{\partial p_1}{\partial \beta} & \frac{\partial p_2}{\partial \beta} & \dots & \frac{\partial p_n}{\partial \beta} \end{bmatrix} \in \mathbb{R}^{(k+1) \times n}$$

$$\frac{\partial p_i}{\partial \beta} = p_i(1-p_i) x_i$$

$$\Rightarrow \frac{\partial \mathbf{p}}{\partial \beta} = \begin{bmatrix} p_1(1-p_1)x_1 & p_2(1-p_2)x_2 & \dots & p_n(1-p_n)x_n \end{bmatrix}$$
$$= \mathbf{X}^T \mathbf{W}$$
$$\mathbf{W} = \begin{bmatrix} p_1(1-p_1) & & & 0 \\ & p_2(1-p_2) & & \\ 0 & & \ddots & \\ & & & p_n(1-p_n) \end{bmatrix}$$

$$\Rightarrow \mathbf{H}(\beta) = -\mathbf{X}^T \mathbf{W} \mathbf{X}$$

(diagonal matrix)

Putting everything together

Want to maximize the log likelihood $\ell(\beta|\mathbf{y}, \mathbf{X})$.

• begin with initial guess $\beta^{(0)}$

• update:

$$\beta^{(r+1)} = \beta^{(r)} + (X^T W^{(r)} X)^{-1} X^T (y - p^{(r)})$$

$$p_i^{(r)} = \frac{e^{x_i^T \beta^{(r)}}}{1 + e^{x_i^T \beta^{(r)}}}$$

$$p^{(r)} = (p_1^{(r)}, \dots, p_n^{(r)})^T$$

$$W^{(r)} = \text{diag} (p_i^{(r)} (1 - p_i^{(r)}))$$

Class activity

Work on the class activity:

https://sta711-s26.github.io/class_activities/ca_07_2.html

Submit your work on Canvas.